Fix kv proof

src/program_proof/simplepb/apps/kv_proof.v
@@ -4,57 +4,108 @@ From Perennial.program_proof Require Import marshal_stateless_proof.
 From iris.base_logic Require Import ghost_map.
 From Perennial.goose_lang Require Import crash_borrow.
 From Perennial.program_proof.simplepb.simplelog Require Import proof.
-From Perennial.program_proof.simplepb Require Import pb_definitions.
+From Perennial.program_proof.simplepb Require Import pb_definitions config_proof.
 From Perennial.program_proof.simplepb Require Import pb_apply_proof clerk_proof.
 From Perennial.program_proof.grove_shared Require Import erpc_lib.
 From Perennial.program_proof Require Import map_marshal_proof.
 From Perennial.program_proof Require Import map_marshal_proof.
 From iris.algebra Require Import dfrac_agree mono_list.
 
-From Perennial.program_proof.simplepb.apps Require Import esm_proof kv_vsm_proof log.
+From Perennial.program_proof.simplepb.apps Require Import vsm esm_proof kv_vsm_proof log.
 
-Section global_proof.
+Class kvG Σ := KvG {
+  kv_ghostMapG :> ghost_mapG Σ string string ;
+  kv_logG :> inG Σ (mono_listR (leibnizO kvOp)) ;
+  kv_vsmG :> vsmG (sm_record:=kv_record) Σ ;
+}.
+Definition kvΣ := #[configΣ; ghost_mapΣ string string;
+                      GFunctor (mono_listR (leibnizO kvOp));
+                      vsmΣ (sm_record:=kv_record)
+   ].
+Global Instance subG_kvΣ {Σ} : subG kvΣ Σ → kvG Σ.
+Proof. intros. solve_inG. Qed.
 
-Definition eekv_record := (ee_record (low_record:=kv_record)).
+Definition ekv_record := (esm_record (low_record:=kv_record)).
 Class ekvG Σ :=
   {
     ekv_erpcG :> erpcG Σ (list u8) ;
-    ekv_simplelogG :> simplelogG (sm_record:=eekv_record) Σ;
-    ekv_kvG :> kv64G Σ ;
+    ekv_simplelogG :> simplelogG (sm_record:=ekv_record) Σ;
+    ekv_kvG :> kvG Σ ;
   }.
 
-Definition ekvΣ := #[erpcΣ (list u8); simplelogΣ (sm_record:=eekv_record);
-                     kv64Σ].
+Definition ekvΣ := #[erpcΣ (list u8); simplelogΣ (sm_record:=ekv_record);
+                     kvΣ].
 Global Instance subG_ekvΣ {Σ} : subG ekvΣ Σ → ekvG Σ.
 Proof. intros. solve_inG. Qed.
 
-Context `{!ekvG Σ, !gooseGlobalGS Σ}.
+Section global_proof.
+
+
+Context `{!gooseGlobalGS Σ}.
+Context `{!ekvG Σ}.
+
+(* The abstract state applies the operation to an all-nil map,
+   so that each key already exists from the start. This is consisent with
+   [getOp] doing [default []]. *)
+Definition own_kvs (γkv:gname) ops : iProp Σ :=
+  ∃ allocatedKeys,
+  ghost_map_auth γkv 1 (compute_state ops ∪ gset_to_gmap "" allocatedKeys)
+.
+
+Definition stateN := nroot .@ "state".
+
+Definition kv_inv γlog γkv : iProp Σ :=
+  inv stateN ( ∃ ops, own_log γlog ops ∗ own_kvs γkv ops).
+
+Definition kv_ptsto γkv (k v : string) : iProp Σ :=
+  k ↪[γkv] v.
+
+Lemma alloc_kv γlog allocated :
+  own_log γlog [] ={⊤}=∗
+  ∃ γkv ,
+  kv_inv γlog γkv ∗
+  [∗ set] k ∈ allocated, kv_ptsto γkv k ""
+.
+Proof.
+  iIntros "Hlog".
+  iMod (ghost_map_alloc (gset_to_gmap "" allocated)) as (γkv) "[Hkvs Hkvptsto]".
+  iExists _.
+  iMod (inv_alloc with "[Hkvs Hlog]") as "$".
+  { iNext. iExists _; iFrame. rewrite /own_kvs /compute_state /=.
+    iExists _. rewrite left_id_L. done. }
+  replace allocated with (dom (gset_to_gmap "" allocated)) at 2.
+  2:{ rewrite dom_gset_to_gmap. done. }
+  iApply big_sepM_dom. iApply (big_sepM_impl with "Hkvptsto").
+  iIntros "!# %k %x".
+  rewrite lookup_gset_to_gmap_Some.
+  iIntros ([_ <-]). auto.
+Qed.
 
 (* These are the client-side invs *)
 Definition is_ekv_invs γpb γkv : iProp Σ :=
   ∃ γlog γerpc,
-  is_ee_inv (low_record:=kv_record) γpb γlog γerpc ∗
+  is_esm_inv (low_record:=kv_record) γpb γlog γerpc ∗
   is_eRPCServer γerpc ∗
   kv_inv γlog γkv
 .
 
 Definition is_kv_config confHost γkv : iProp Σ :=
   ∃ γpb γerpc γlog,
-    "#Hee_inv" ∷ is_ee_inv (low_record:=kv_record) γpb γlog γerpc ∗
+    "#Hee_inv" ∷ is_esm_inv (low_record:=kv_record) γpb γlog γerpc ∗
     "#Herpc_inv" ∷ is_eRPCServer γerpc ∗
     "#Hkv_inv" ∷ kv_inv γlog γkv ∗
     "#Hconf" ∷ is_pb_sys_host confHost γpb
 .
 
-Lemma alloc_ekv γpb :
+Lemma alloc_ekv γpb allocated :
   own_op_log γpb [] ={⊤}=∗
   ∃ γkv ,
   is_ekv_invs γpb γkv ∗
-  [∗ set] k ∈ fin_to_set u64, kv_ptsto γkv k []
+  [∗ set] k ∈ allocated, kv_ptsto γkv k ""
 .
 Proof.
   iIntros "Hoplog".
-  iMod (alloc_ee with "[$]") as (??) "(#? & #? & ?)".
+  iMod (alloc_esm with "[$]") as (??) "(#? & #? & ?)".
   iMod (alloc_kv with "[$]") as (?) "(#? & Hkvs)".
   iExists _. iFrame.
   iModIntro. repeat iExists _; iFrame "#".
@@ -69,12 +120,11 @@ Context `{!ekvG Σ}.
 
 Lemma wp_Start fname (confHost host:chan) γsys γsrv data :
   {{{
-      "#Hhost" ∷ is_pb_host (pb_record:=eekv_record) host γsys γsrv ∗
+      "#Hhost" ∷ is_pb_host (pb_record:=ekv_record) host γsys γsrv ∗
       "#HconfHost" ∷ config_protocol_proof.is_pb_config_host confHost γsys ∗
       "Hfile_ctx" ∷ crash_borrow (fname f↦ data ∗ file_crash (own_Server_ghost_f γsys γsrv) data)
                   (|C={⊤}=> ∃ data', fname f↦ data' ∗ ▷ file_crash (own_Server_ghost_f γsys γsrv) data') ∗
 
-      (* FIXME: collect these invariants *)
       "#Hinvs" ∷ is_pb_system_invs γsys
   }}}
     Start #(LitString fname) #(host:u64) #(confHost:u64)
@@ -86,15 +136,15 @@ Proof using Type*.
   iIntros (Φ) "Hpre HΦ".
   iNamed "Hpre".
   wp_call.
-  wp_apply (wp_MakeKVStateMachine).
+  wp_apply (wp_makeVersionedStateMachine).
   iIntros (??) "[#His1 Hown]".
-  wp_apply (wp_MakeEEKVStateMachine with "[Hown]").
+  wp_apply (wp_MakeExactlyOnceStateMachine with "[Hown]").
   {
     iFrame.
     iFrame "His1".
   }
   iIntros (??) "[#His2 Hown]".
-  wp_apply (wp_MakePbServer (sm_record:=eekv_record) with "[$Hown $Hfile_ctx]").
+  wp_apply (wp_MakePbServer (sm_record:=ekv_record) with "[$Hown $Hfile_ctx]").
   { iFrame "#". }
   iIntros (?) "His".
   wp_pures.
@@ -105,16 +155,16 @@ Qed.
 
 Definition own_Clerk ck γkv : iProp Σ :=
   ∃ (eeCk:loc) γlog,
-    "Hcl" ∷ ck ↦[kvee.Clerk :: "cl"] #eeCk ∗
+    "Hcl" ∷ ck ↦[kv.Clerk :: "cl"] #eeCk ∗
     "#Hkvinv" ∷ kv_inv γlog γkv ∗
-    "Hownck" ∷ eesm_proof.own_Clerk (low_record:=kv_record) eeCk γlog
+    "Hownck" ∷ esm_proof.own_Clerk (low_record:=kv_record) eeCk γlog
 .
 
 Lemma wp_MakeClerk γkv confHost :
   {{{
       is_kv_config confHost γkv
   }}}
-    kvee.MakeClerk #confHost
+    kv.MakeClerk #confHost
   {{{
         ck, RET #ck; own_Clerk ck γkv
   }}}
@@ -123,7 +173,7 @@ Proof.
   iIntros (Φ) "Hpre HΦ".
   iNamed "Hpre".
   wp_call.
-  wp_apply (eesm_proof.wp_MakeClerk with "[]").
+  wp_apply (esm_proof.wp_MakeClerk with "[]").
   { iFrame "#". }
   iIntros (?) "Hck".
   wp_apply (wp_allocStruct).
@@ -136,14 +186,14 @@ Proof.
   iFrame "∗#".
 Qed.
 
-Lemma wp_Clerk__Put ck γkv key val_sl value :
-⊢ {{{ own_Clerk ck γkv ∗ own_slice_small val_sl byteT 1 value }}}
+Lemma wp_Clerk__Put ck γkv key value :
+⊢ {{{ own_Clerk ck γkv }}}
   <<< ∀∀ old_value, kv_ptsto γkv key old_value >>>
-    Clerk__Put #ck #key (slice_val val_sl) @ (↑pbN ∪ ↑prophReadN ∪ ↑eeN ∪ ↑stateN)
+    Clerk__Put #ck #(str key) #(str value) @ (↑pbN ∪ ↑prophReadN ∪ ↑esmN ∪ ↑stateN)
   <<< kv_ptsto γkv key value >>>
   {{{ RET #(); own_Clerk ck γkv }}}.
 Proof.
-  iIntros "%Φ !# [Hck Hval_sl] Hupd".
+  iIntros "%Φ !# Hck Hupd".
   wp_lam.
   wp_pures.
   wp_apply (wp_allocStruct).
@@ -153,7 +203,7 @@ Proof.
   iNamed "HH".
   wp_pures.
   iNamed "Hck".
-  wp_apply (wp_EncodePutArgs with "[$Key $Val $Hval_sl]").
+  wp_apply (wp_encodePutArgs with "[$Key $Val]").
   iIntros (putEncoded put_sl) "[%Henc Henc_sl]".
   wp_loadField.
   wp_apply (wp_Clerk__ApplyExactlyOnce with "Hownck Henc_sl").
@@ -173,6 +223,7 @@ Proof.
   iExists _; iFrame.
   iIntros "Hlog".
 
+  iNamed "Hkvs".
   iMod (ghost_map_update (value) with "Hkvs Hkvptsto") as "[Hkvs Hkvptsto]".
 
   iMod ("Hkvclose" with "Hkvptsto") as "HH".
@@ -185,6 +236,7 @@ Proof.
     unfold compute_state.
     rewrite foldl_snoc.
     simpl. rewrite insert_union_l.
+    iExists _.
     iFrame.
   }
   iModIntro.
@@ -199,15 +251,15 @@ Qed.
 Lemma wp_Clerk__Get ck γkv key :
 ⊢ {{{ own_Clerk ck γkv }}}
   <<< ∀∀ value, kv_ptsto γkv key value >>>
-    Clerk__Get #ck #key @ (↑pbN ∪ ↑prophReadN ∪ ↑eeN ∪ ↑stateN)
+    Clerk__Get #ck #(str key) @ (↑pbN ∪ ↑prophReadN ∪ ↑esmN ∪ ↑stateN)
   <<< kv_ptsto γkv key value >>>
-  {{{ reply_sl, RET (slice_val reply_sl); own_Clerk ck γkv ∗ own_slice_small reply_sl byteT 1 value }}}.
+  {{{ RET #(str value); own_Clerk ck γkv }}}.
 Proof.
   iIntros "%Φ !# Hck Hupd".
   wp_lam.
   wp_pures.
   iNamed "Hck".
-  wp_apply (wp_EncodeGetArgs with "[//]").
+  wp_apply (wp_encodeGetArgs with "[//]").
   iIntros (getEncoded get_sl) "[%Henc Henc_sl]".
   wp_loadField.
   wp_apply (wp_Clerk__ApplyReadonly with "Hownck Henc_sl").
@@ -227,24 +279,28 @@ Proof.
   iExists _; iFrame "Hlog".
   iIntros "Hlog".
 
+  iNamed "Hkvs".
   iDestruct (ghost_map_lookup with "[$] [$]") as %Hlook.
 
-  iMod ("Hkvclose" with "Hkvptsto") as "HH".
+  iMod ("Hkvclose" with "Hkvptsto") as "HΦ".
   iMod "Hmaskclose" as "_".
   iMod ("Hclose" with "[Hlog Hkvs]") as "_".
-  { iExists _; iFrame. }
+  { iExists _; iFrame. iExists _; iFrame. }
   iModIntro.
-  iIntros (?) "Hsl Hck".
-  iApply "HH".
-  iSplitR "Hck".
-  { repeat iExists _. iFrame "∗#". }
-  { rewrite /kv_record//=. move:Hlook.
-    rewrite lookup_union.
-    destruct (compute_state ops !! key) as [x|]; simpl.
-    - rewrite union_Some_l. intros [= ->]. done.
-    - rewrite left_id lookup_gset_to_gmap option_guard_True.
-      2:{ apply elem_of_fin_to_set. }
-      intros [= ->]. done. }
+  iIntros (?) "Hck Hsl".
+  wp_apply (wp_StringFromBytes with "[$]").
+  iIntros "_".
+  simpl. rewrite string_to_bytes_inj /=.
+  rewrite lookup_union in Hlook.
+  destruct (compute_state ops !! key) as [x|]; simpl.
+  - simpl in Hlook. rewrite union_Some_l in Hlook.
+    injection Hlook as <-.
+    iApply "HΦ". repeat iExists _. iFrame "∗#".
+  -
+    Search lookup gset_to_gmap.
+    rewrite left_id lookup_gset_to_gmap_Some in Hlook.
+    destruct Hlook as [? ?]; subst.
+    iApply "HΦ". repeat iExists _. iFrame "∗#".
 Qed.
 
 End local_proof.
